\documentclass[../../RotatingBosons.tex]{subfiles}

\begin{document}

%%%%%%%%%%%%%%%%%%%%%%%%%%%%%%%%%%%%%%%%
%%%%%%%%%%%%%%%%%%%%%%%%%%%%%%%%%%%%%%%%
%%%%%%%%%%% ANALYTICAL SOLUTIONS %%%%%%%%%%%%%%%
%%%%%%%%%%%%%%%%%%%%%%%%%%%%%%%%%%%%%%%%
%%%%%%%%%%%%%%%%%%%%%%%%%%%%%%%%%%%%%%%%

\section{\label{NRRBchecks}NOT UPDATED YET:Some checks on our code}
\subsection{Nonrotating, noninteracting, nonrelativistic, finite chemical potential in 1, 2, and 3 dimensions}
The lattice action for a nonrotating, noninteracting, and nonrelativistic system is the following:
\beq
S_{\text{lat},r} = \phi_{r}^{*}\left[\phi_{r} - e^{d\tau\mu} \phi_{r - \hat{\tau}} - \frac{d\tau}{2m}\sum_{i =1}^{d}\left(  \phi_{r + \hat{i}} - 2 \phi_{r} + \phi_{r - \hat{i}}\right) \right].
\eeq
This can be written as fields multiplying a matrix:
\beq
S_{\text{lat},r} = \sum_{r}\sum_{r'}\phi_{r}^{*}M\phi_{r'} = \sum_{r}\sum_{r'}\phi_{r}^{*}\left[ (1 + \frac{d\tau d}{m})\delta_{r,r'}  - e^{d\tau\mu} \delta_{r - \hat{\tau},r'}- \frac{d\tau}{2m}\sum_{i =1}^{d}\left(\delta_{r+\hat{i},r'} + \delta_{r-\hat{i},r'} \right)\right]\phi_{r'},
\eeq
which we can use to determine analytically the density and field modulus squared of this system in order to check against our code's results. Recall that
\bea
\left \langle \hat{n} \right \rangle & = & \frac{-1}{V}\frac{\partial ln \CZ}{\partial (\beta \mu)} = \frac{-1}{V}\frac{\partial}{\partial (\beta\mu)} (-ln(det(M))) \\
& = & \frac{1}{V}\frac{\partial}{\partial (\beta\mu)}Tr(ln M) = \frac{1}{V}\frac{\partial}{\partial (\beta\mu)}\sum_{k}ln D_{kk} = \frac{1}{V}\sum_{k}\frac{1}{D_{kk}}\frac{\partial D_{kk}}{\partial (\beta\mu)}\nonumber
\eea with $\beta \mu = N_{\tau} d\tau \mu$, and note that for a nonrelativistic system,
%
\bea
\left \langle \phi^{*}\phi \right \rangle & =& \frac{-1}{V}\frac{\partial ln \CZ}{\partial  (d/m)} = \frac{-1}{V}\frac{\partial}{\partial  (d/m)} (-ln(det(M))) \\
& =& \frac{1}{V}\frac{\partial}{\partial (d/m)}Tr(ln M) = \frac{1}{V}\frac{\partial}{\partial  (d/m)}\sum_{k}ln D_{kk} \nonumber \\
&= &\frac{1}{V}\sum_{k}\frac{1}{D_{kk}}\frac{\partial D_{kk}}{\partial  (d/m)} = \sum_{k}\frac{1}{D_{kk}}. \nonumber
\eea
%
\subsubsection{Diagonalizing our matrix, M}
We can represent the nonrotating, noninteracting action as
\beq
S[\lambda = \omega = 0] = \sum_{r,r'}\phi^{*}_{r}M_{r,r'}[d,m,\mu]\phi_{r'}
\eeq
where 
\beq
M_{r,r'}[d,m,\mu] = \left[ (1+\frac{d\tau d}{m})\delta_{r,r'} - e^{d\tau\mu}\delta_{r-\hat{t},r'}-\frac{d\tau}{2m}\sum_{i=1}^{d}(\delta_{r+\hat{i},r'}+\delta_{r-\hat{i},r'})\right].
\eeq 
We want to diagonalize $M$ by applying a transformation matrix, such that $D_{kk'} = U^{\dagger}MU$, where
\bea
U_{r,k}& =& \frac{\sqrt{2^{d}}}{\sqrt{N_{x}^{d} N_{\tau}}}e^{i k_{0} t}\prod_{i=1}^{d}\sin(k_{i}x_{i}) \\
U^{\dagger}_{r,k}& =& \frac{\sqrt{2^{d}}}{\sqrt{N_{x}^{d} N_{\tau}}}e^{-i k_{0} t}\prod_{i=1}^{d}\sin(k_{i}x_{i}) \\
k_{0} & = & \frac{2 \pi n_{0}}{N_{\tau}},\ n_{0} \in [1,2,...,N_{\tau}] \\
k_{i} & = & \frac{\pi n_{i}}{(N_{x}+1)},\ n_{i} \in [1,2,...,N_{x}].
\eea
Applying the transformation matrix, we get
\bea
D_{k,k'} &=& \frac{2^{d}}{N_{x}^{d} N_{t}}\sum_{r,r'}e^{-i k_{0} t}\prod_{i=1}^{d}\sin(k_{i}x_{i})\left[ (1+\frac{d\tau d }{m})\delta_{r,r'} \right]e^{i k'_{0} t'}\prod_{i=1}^{d}\sin(k'_{i}x'_{i})\nonumber \\
&& -\frac{2^{d}}{N_{x}^{d} N_{t}}\sum_{r,r'}e^{-i k_{0} t}\prod_{i=1}^{d}\sin(k_{i}x_{i})\left[e^{ d\tau \mu}\delta_{r-\hat{t},r'}\right]e^{i k'_{0} t'}\prod_{i=1}^{d}\sin(k'_{i}x'_{i})  \\
&& -\frac{2^{d}}{N_{x}^{d} N_{t}}\sum_{r,r'}e^{-i k_{0} t}\prod_{i=1}^{d}\sin(k_{i}x_{i})\left[\frac{d\tau}{2m} \sum_{i=1}^{d}\delta_{r+\hat{i},r'}\right]e^{i k'_{0} t'}\prod_{i=1}^{d}\sin(k'_{i}x'_{i})\nonumber\\
&& -\frac{2^{d}}{N_{x}^{d} N_{t}}\sum_{r,r'}e^{-i k_{0} t}\prod_{i=1}^{d}\sin(k_{i}x_{i})\left[\frac{d\tau}{2m}\sum_{i=1}^{d}\delta_{r-\hat{i},r'}\right]e^{i k'_{0} t'}\prod_{i=1}^{d}\sin(k'_{i}x'_{i})\nonumber.
\eea
Resolving the delta functions, performing the sum over $r'$, and pulling everything that does not depend on $r = (t,\vec{x})$ outside the sum, this reduces to
\bea
D_{k,k'} &=& \frac{2^{d}}{N_{x}^{d} N_{t}} (1+\frac{d\tau d}{m})\sum_{r}e^{-i t(k_{0} -k'_{0})}\prod_{i=1}^{d}\sin(k_{i}x_{i})\sin(k'_{i}x_{i})\nonumber \\
&& -\frac{2^{d}}{N_{x}^{d} N_{t}}e^{d\tau\mu}e^{-ik'_{0}}\sum_{r}e^{-i t(k_{0}- k'_{0})}\prod_{i=1}^{d}\sin(k_{i}x_{i})\sin(k'_{i}x_{i})  \\
&& -\frac{2^{d}}{N_{x}^{d} N_{t}}\frac{d\tau}{2m}\sum_{r}e^{-i t(k_{0} -k'_{0})}\prod_{i=1}^{d}\sin(k_{i}x_{i})\sum_{i=1}^{d}\sin(k'_{i}x_{i}+k'_{i})\nonumber\\
&& -\frac{2^{d}}{N_{x}^{d} N_{t}}\frac{d\tau}{2m}\sum_{r}e^{-i t(k_{0} -k'_{0})}\prod_{i=1}^{d}\sin(k_{i}x_{i}) \sum_{i=1}^{d}\sin(k'_{i}x_{i}-k'_{i})\nonumber.
\eea
To further expand the last two lines, we use the following trig identity: $\sin(a \pm b) = \sin(a)\cos(b) \pm \sin(b)\cos(a)$, which gives us:
\bea
D_{k,k'} &=& \frac{2^{d}}{N_{x}^{d} N_{t}} (1+\frac{ d\tau d}{m} -e^{d\tau\mu}e^{-ik'_{0}} )\sum_{r}e^{-i t(k_{0} -k'_{0})}\prod_{i=1}^{d}\sin(k_{i}x_{i})\sin(k'_{i}x_{i}) \\
&& -\frac{2^{d}}{N_{x}^{d} N_{t}}\frac{d\tau}{2m}\sum_{i=1}^{d}\cos(k'_{i})\sum_{r}e^{-i t(k_{0} -k'_{0})}\prod_{i=1}^{d}\sin(k_{i}x_{i})\sin(k'_{i}x_{i})\nonumber\\
&& -\frac{2^{d}}{N_{x}^{d} N_{t}}\frac{d\tau}{2m}\sum_{i=1}^{d}\sin(k'_{i})\sum_{r}e^{-i t(k_{0} -k'_{0})}\prod_{i=1}^{d}\sin(k_{i}x_{i})\cos(k'_{i}x_{i})\nonumber\\
&& -\frac{2^{d}}{N_{x}^{d} N_{t}}\frac{d\tau}{2m}\sum_{i=1}^{d}\cos(k'_{i})\sum_{r}e^{-i t(k_{0} -k'_{0})}\prod_{i=1}^{d}\sin(k_{i}x_{i}) \sin(k'_{i}x_{i})\nonumber\\
&& +\frac{2^{d}}{N_{x}^{d} N_{t}}\frac{d\tau}{2m} \sum_{i=1}^{d}\sin(k'_{i})\sum_{r}e^{-i t(k_{0} -k'_{0})}\prod_{i=1}^{d}\sin(k_{i}x_{i})\cos(k'_{i}x_{i})\nonumber.
\eea
Using the following Fourier identities
\bea
\sum_{x}\sin(kx)\sin(k'x) & = &\frac{N_{x}}{2}\delta_{k,k'}\nonumber\\
\sum_{x}\sin(kx)\cos(k'x) & = &0 \\
\sum_{x}e^{-i x (k-k')} &=& N_{x}\delta_{k,k'}\nonumber\\
\eea we find that
\bea
D_{k,k'} &=& \frac{2^{d}}{N_{x}^{d} N_{t}} \left(1+\frac{d\tau d}{m} -e^{d\tau\mu}e^{-ik'_{0}} -\frac{d\tau}{m}\sum_{i=1}^{d}\cos(k'_{i})\right)N_{t}\delta_{k_{0},k'_{0}}\prod_{i=1}^{d}\frac{N_{x_{i}}}{2} \delta_{k_{i},k'_{i}}\nonumber\\
&=& \frac{2^{d}}{N_{x}^{d} N_{t}} \left(1+\frac{ d\tau d}{m} -e^{ d\tau\mu}e^{-ik'_{0}} -\frac{d\tau}{m}\sum_{i=1}^{d}\cos(k'_{i})\right)N_{t}\left(\frac{N_{x}}{2}\right)^{d} \delta_{k,k'}\nonumber\\
D_{k,k'} &=& \left(1+\frac{d\tau d}{m} -e^{d\tau\mu}e^{-ik'_{0}} -\frac{d\tau}{m}\sum_{i=1}^{d}\cos(k'_{i})\right) \delta_{k,k'}\nonumber,
\eea
or, slightly rearranged:
\beq
D_{k,k'} = \left(1 -e^{ d\tau\mu}e^{-ik'_{0}} +\frac{d\tau}{m}\sum_{i=1}^{d}(1-\cos(k'_{i}))\right) \delta_{k,k'}.
\eeq
Note that this is a complex matrix, with real and imaginary parts:
\bea
\text{Re}\left[D_{k,k'}\right] &=&  \left(1 -e^{ d\tau\mu}\cos(k'_{0}) +\frac{d\tau}{m}\sum_{i=1}^{d}(1-\cos(k'_{i}))\right) \delta_{k,k'} \\
\text{Im}\left[D_{k,k'}\right] &=&  e^{ d\tau\mu}\sin(k'_{0}) \delta_{k,k'} .
\eea

\subsubsection{Analytical solution for the nonrotating, noninteracting density}
We can now use our diagonal matrix $D_{k,k'} = D_{k,k}$ to solve for the density of this system. Recall that
\beq
\left \langle \hat{n} \right \rangle = \frac{1}{V N_{\tau}}\sum_{k}\frac{1}{D_{kk}}\frac{\partial D_{kk}}{\partial (d\tau\mu)}.
\eeq
We first need to solve for $\frac{\partial D_{kk}}{\partial (d\tau\mu)}$:
\bea
\frac{\partial D_{kk}}{\partial \mu} & = & \frac{\partial}{\partial (d\tau\mu)}\left[ \left(1 -e^{d\tau\mu}e^{-ik'_{0}} +\frac{d\tau}{m}\sum_{i=1}^{d}(1-\cos(k'_{i}))\right) \delta_{k,k'}\right] \\ \nonumber
& = & - e^{d\tau\mu}e^{-ik'_{0}}\delta_{k,k'}.
\eea Plugging this in to our equation for the density gives us:
\beq
\left \langle \hat{n} \right \rangle = \frac{1}{N_{x}^{d}N_{t}}\sum_{k}\frac{D^{*}_{kk}}{|D_{kk}|^{2}}\left( -e^{d\tau\mu}e^{-ik'_{0}}\delta_{k,k'}\right).
\eeq

\subsubsection{Analytical solution for the nonrotating, noninteracting field modulus squared}
\beq
\left \langle \phi^{*}\phi \right \rangle  = \sum_{k}\frac{1}{D_{kk}} = \sum_{k}\frac{D^{*}_{kk}}{|D_{kk}|^{2}}.
\eeq


\subsubsection{Analytical solution for the two-point correlation function}
The eigenvalues and eigenvectors can be used to compute the solution for two-point correlation function for this system:
\beq
G(x, x') = \sum_{k} \frac{1}{D_{kk}}U^{\dagger}_{k}(x)U_{k}(x')
\eeq

\end{document}